\documentclass{article}
\input{preamble.tex}

\begin{document}
\section{Lecture 12}
\subsection{Identities Between Operations}

We have seen three operations defined by \( \nabla \).

\[ \text{Gradient: } \nabla f, \quad \text{Divergence: } \nabla \cdot  \vec{F}, \quad \text{Curl: } \nabla \times  \vec{F} \]

There are many identities, we'll now look at one.

\begin{prop}
	For any scalar field \( f \), we have

	\[ \nabla \times  \left( \nabla f \right)=0 \]
\end{prop}

\begin{proof}
	We have \( \nabla f = \left( f_{x},f_{y},f_{z} \right) \), then

	\[ \nabla \times \left( \nabla f \right) =
		\left|\begin{bmatrix}
			\vec{i}    & \vec{j}    & \vec{k}    \\
			\partial_x & \partial_y & \partial_z \\
			f_{x}      & f_{y}      & f_{z}
		\end{bmatrix}\right| = \left( f_{zy}-f_{yz}, -f_{zx}+f_{xz},f_{yx} - f_{xy} \right)\]

	But partial derivatives can be exchanged. Then we find that \( \nabla \times \left( \nabla f \right)= 0 \)
\end{proof}

We are going to use this when we discuss conservative fields.

\subsection{Line Integrals}

Consider the curve \( C \) with

\[ \vec{r}\left( t \right)= \left( x\left( t \right),y\left( t \right) \right), t_{0} \leq t \leq t_{1}  \]


\begin{figure}[H]
	\centering
	\incfig[0.8]{lineintegrals}
\end{figure}

\[ \Delta x = x\left( t+\Delta t \right)-x\left( t \right), \quad \Delta y = y\left( t+\Delta t \right)-y\left( t \right) \]

The distance between the two points is

\[ \Delta S = \sqrt{\left( \Delta x^2\right) + \left( \Delta y \right)^2 } \]

When \( \Delta t  \) is small, we can use the following approximation

\[ \Delta x \approx \frac{d x}{dt}\Delta t ,\quad \Delta y \approx \frac{d y}{dt}\Delta t \]

Then, for the distance, we get

\[ S = \sqrt{\left( \frac{d x}{dt}\Delta t^2 \right)+\left( \frac{d y}{dt}\Delta t^2 \right)}=\Delta t \sqrt{\left( \frac{d x}{dt} \right)^2+\left( \frac{d y}{dt} \right)^2} \]

Letting \( \Delta t \rightarrow 0 \) leads to the following

\begin{definition}
	The line integral of \( f\left( x,y \right) \) along a curve \( C \) is defined by

	\[ \int_{C}fds = \int_{t_{0} }^{t_{1} } f\left( x\left( t \right),y\left( t \right) \right)\sqrt{x'\left( t \right)^2+y'\left( t \right)^2} dt \]
\end{definition}

\begin{observe}
	Note that \( f \) is restricted to \( \vec{r}\left( t \right)=\left( x\left( t \right),y\left( t \right) \right) \). When \( f=1 \), we recover the arc length.
\end{observe}

\begin{eg}
	Consider \( C \) defined by

	\[ x\left( t \right)=t, \quad y\left( t \right)=0, \quad 0 \leq t \leq 1 \]

	\begin{figure}[H]
		\centering
		\incfig[0.8]{f12eg1}
	\end{figure}

	First, we compute

	\[ \sqrt{x'\left( t \right)^2 + y'\left( t \right)^2}dt = \sqrt{1^2+0^2}=1 \]

	Now, consider \( f\left( x,y \right)=x^2+y \). We want to compute \( \int_{C}fds \). Restricting \( f \) to \( C \) gives

	\[ f\left( x\left( t \right),y\left( t \right) \right) = x\left( t \right)^2+y\left( t \right)^2 = t^2+0 = t^2 \]

	Then we obtain

	\[ \int_{C}fds=\int_{0}^{1} t^2 \cdot 1 dt=\frac{1}{3}  \]
\end{eg}

\begin{note}
	Line integrals can be used to compute the mass of a 1-dimensional object. The curve \( C \) describes the object, and the function \( \int_{C}fds \) is the mass.

	\begin{figure}[H]
		\centering
		\incfig[0.4]{f12note1}
	\end{figure}
\end{note}

\subsection{Parametrization and Orientation}
The next result is as for the arc length.

\begin{prop}
	The integral \( \int_{C}fds \) does not depent on the parametrization of \( C \).
\end{prop}

We will consider a special case

\begin{eg}
	Consider \( C \) with

	\[ \vec{r}\left( t \right)=\left( x\left( t \right),y\left( t \right) \right), t_{0} \leq t \leq t_{1}  \]

	We have

	\[ \text{Start: } A = \left( x\left( t_{0}  \right), y \left( t_{0}  \right) \right), \quad \text{End: } B = \left( x\left( t_{1}  \right), y\left( t_{1}  \right) \right) \]

	We want to go from \( B \) to \( A \).


	\begin{figure}[H]
		\centering
		\incfig{f12eg2}
	\end{figure}

	We can do this in the following manner

	\[ \vec{r}_{\text{opp}}=\left( x\left( -t \right),y\left( -t \right) \right), \quad -t_{1} \leq t \leq -t_{0}  \]


	Note that
	\begin{align*}
		 & \vec{r}_{\text{opp}}\left( -t_{1}  \right)= \left( x\left( t1 \right),y\left( t_{1}  \right) \right) = B \\
		 & \vec{r}_{\text{opp}}\left( -t_{0}  \right)= \left( x\left( t0 \right),y\left( t_{0}  \right) \right) = A \\
	\end{align*}
\end{eg}

\begin{eg}
	Consider the segment \( C \) from \( \left( 0,0 \right) \) to \( \left( 1,0 \right) \). Take \( f\left( x,y \right)=x \). Show that \( \int_{C}fds=\frac{1}{2}  \) using \( \vec{r}\left( t \right) \) and \( \vec{r}_{\text{opp}}\left( t \right) \).

	If \( C \) parametrized by \( \vec{r}\left( t \right) \), we use \( -C \) when considering \( \vec{r}_{\text{opp}}\left( t \right) \). We have

	\[ \int_{C}fds=\int_{-C}fds \]

	The situation will be different for vector fields.
\end{eg}

\subsection{Case of Vector Fields}

Consider the curve with

\begin{align*}
	 & \vec{r}\left( t \right)=\left( x\left( t \right),y\left( t \right) \right), \quad t_{0} \leq t \leq t_{1}     \\
	 & \vec{r'} \left( t \right)=\left( x'\left( t \right),y'\left( t \right) \right) \quad \text{(Velocity vector)}
\end{align*}

\begin{definition}
	The line integral of \( \vec{F} \) along \( C \) is

	\[ \int_{C}\vec{F} \cdot d\vec{r}= \int_{t_{0} }^{t_{1} } \vec{F}\left( \vec{r}\left( t \right) \right) \cdot \vec{r}' dt \]

	Here \( \vec{F}\left( \vec{r}\left( t \right) \right) = \vec{F}\left( x\left( t \right),y\left( t \right) \right) \)
\end{definition}

In physics, we have that \( \vec{F} \) is the force, and \( \int_{C}\vec{F}d \vec{r} \) is the work done by \( \vec{F} \) along \( C \). The elementary case is given by \( W = FS \), or work = force \(  \cdot  \) displacement. More explicitly, we consider

\[ \vec{F}\left( x,y \right)=\left( P\left( x,y \right),Q\left( x,y \right) \right)  \]

Then we have

\[ \vec{F}\left( \vec{r}\left( t \right) \right) \cdot \vec{r}'\left( t \right)= P\left( x\left( t \right),y\left( t \right) \right) \cdot x'\left( t \right)+Q\left( x\left( t \right),y\left( t \right) \right) \cdot  y'\left( t \right) \]

The line integral is then

\[ \int_{C}\vec{F} \cdot d \vec{r} = \int_{t_{0} }^{t_{1} } P\left( x\left( t \right),y\left( t \right) \right) \cdot  x'\left( t \right) dt + \int_{t_{0} }^{t_{1} } Q\left( x\left( t \right),y\left( t \right) \right) \cdot y'\left( t \right) dt \]

We will write the expression as

\[ \int_{C}\vec{F} \cdot d \vec{r} = \int_{C}P dx + \int_{C} Q dy \]

\begin{eg}
	Consider the curve \( C \) with

	\[ \vec{r}\left( t \right)=\left( t,t^2 \right), \quad 0 \leq t \leq 1 \]

	\begin{figure}[H]
		\centering
		\incfig[1]{f12eg3}
	\end{figure}

	We have \( x\left( t \right)=t \) and \( y\left( t \right)=t^2 \), its derivative is

	\[ \vec{r}\left( t \right)=\left( x'\left( t \right),y'\left( t \right) \right)=\left( 1,2t \right) \]

	Now consider the vector field

	\[ \vec{F}\left( x,y \right)=\left( x+y,x \right) \]

	That is \( P = x + y \) and \( Q =x \), when this is restricted to \( C \), we get

	\[ \vec{F}\left( \vec{r}\left( t \right) \right) = \left( x\left( t \right)+y\left( t \right), y\left( t \right) \right) = \left( t+t^2,t \right) \]

	We want to compute

	\[ \vec{F}\left( \vec{r}\left( t \right) \right) \cdot \vec{r}' = \left( t+t^2,t \right) \cdot  \left( 1,2t \right) = \left( 3t^2 + t \right) \]

	We finally obtain

	\[ \int_{C}\vec{F}\cdot d \vec{r} = \int_{0}^{1} \left( 3t^2+t \right) dt = \frac{3}{2}  \]
\end{eg}



\end{document}
