\documentclass{article}
\input{preamble.tex}
\begin{document}
\section{Lecture 15}
\subsection{General Regions (cont.)}
As we saw in the previous lecture, we have the following regions

\begin{figure}[H]
	\centering
	\incfig{ysimple}
	\caption{y-simple}
\end{figure}

\begin{figure}[H]
	\centering
	\incfig{xsimple}
	\caption{x-simple}
\end{figure}

\begin{eg}
	Consider the region with \( -1 \leq x \leq 1 \) and bounder by

	\[ a\left( y \right) = y^2, \quad b\left( y \right)=y^2+\frac{1}{2}  \]


	\begin{figure}[H]
		\centering
		\incfig{examplexsimple}
	\end{figure}

	This is an x-simple region.
\end{eg}

More general regions can be partitioned into x-simple and y-simple regions. A region can be described in many different ways.

\begin{eg}
	Consider the region

	\[ D =\left\{ \left( x,y \right): 0 \leq x \leq 1, \quad -x \leq y \leq x\right\} \]
	\begin{figure}[H]
		\centering
		\incfig{ysimpletriangle}
	\end{figure}
	This is a y-simple region. We can also describe this triangle using x-simple regions.


	\begin{figure}[H]
		\centering
		\incfig{xsimpletriangle}
	\end{figure}

	We have two regions:

	\begin{align*}
		 & D_{1} = \left\{ \left( x,y \right): y \leq x \leq 1, \quad 0 \leq y \leq 1 \right\}   \\
		 & D_{2} = \left\{ \left( x,y \right): -y \leq x \leq 1, \quad -1 \leq y \leq 0 \right\}
	\end{align*}

	We have that \( D = D_{1} \cup D_{2}  \), and

	\[ \iint_{D}fdA = \iint_{D_{1} }fdA + \iint_{D_{2} } fdA \]
\end{eg}

\subsection{Integrations in polar coordinates}

We want to compute \( \iint_{D}fdA  \) using the polar coordinates \( \left( r, \theta \right) \), recall that

\[ x = r \cos \theta, \quad y = r \sin \theta \]

In cartesian coordinates, we use the "infinitesimal area \( dA = dxdy \)". We will now consider small polar regions.


\begin{figure}[H]
	\centering
	\incfig{polarregions}
\end{figure}

Recall that area is equal to \( \frac{1}{2} \theta r^2 \).

\begin{align*}
	\Delta A & = \text{"Large region"} - \text{"Small Region"}                                           \\
	         & = \frac{1}{2} \Delta \theta \left( r + \Delta r \right)^2 - \frac{1}{2} \Delta \theta r^2 \\
	         & = r\Delta\theta r + \frac{1}{2} \Delta \theta \left( \Delta r \right)^2
\end{align*}

Neglecting th \( \left( \Delta r \right)^2 \) term, we get

\[ \Delta A \approx r\Delta\theta\Delta r \]

\begin{prop}
	Suppose \( R \) is described in polar coordinates by \( a \leq r \leq b \) and \( \alpha \leq \theta \leq \beta \), then

	\[ \iint_{R}fdA = \int_{r=a}^{b} \left[ \int_{\theta=\alpha}^{\beta} f\left( r\cos\theta,r\sin\theta \right)r d\theta \right] dr \]
\end{prop}

Here, \( dA = rd\theta dr \) is the infinitesimal area. Also, \( f\left( r\cos\theta,r\sin\theta \right) \) is simply \( f\left( x,y \right) \) in polar coordinates.

\begin{eg}
	Consider a  disc of radius \( t \). Its area is \( \pi t^2 \)

	\begin{figure}[H]
		\centering
		\incfig{disc}
	\end{figure}

	It is described by \( R = \left\{ \left( 1,\theta \right): 0 \leq r \leq t, 0 \leq \theta \leq 2\pi \right\} \). We compute

	\[ \iint_{R}dA = \int_{0}^{t} \left[ \int_{0}^{2\pi} r d\theta \right] dr  \]

	\begin{align*}
		\iint_{R}dA & = \int_{0}^{t} \left[ \int_{0}^{2\pi} r d\theta \right] dr \\
		            & = 2\pi \int_{0}^{t} r dr                                   \\
		            & = 2\pi \left[ \frac{r^2}{2} \right]_{0}^{t}                \\
		            & = \pi t^2
	\end{align*}

\end{eg}

\begin{eg}
	We have \( R \) as before, we want to compute \( \iint_{R}fdA \) where

	\[ f\left( x,y \right)=x^2+y^2 \]

	Using polar coordinates, we get

	\[ f\left( r\cos\theta,r\sin\theta \right) = r^2\left( \cos\theta \right)+r^2+\left( \sin\theta \right)^2 = r^2 \]

	Our double integral is

	\begin{align*}
		\iint_{R}fdA & = \int_{0}^{t} \int_{0}^{2\pi} f\left( r\cos\theta,r\sin\theta\right)r d\theta dr \\
		             & = \int_{0}^{t} \int_{0}^{2\pi} r^3 d\theta dr                                     \\
		             & = 2\pi \int_{0}^{t} r^3 dr                                                        \\
		             & = 2\pi \frac{1}{4} t^{4}                                                          \\
		             & = \frac{\pi}{2}t^{4}
	\end{align*}
\end{eg}

\subsection{Change in variables}

We want to consider general coordinates \( \left( u,v \right) \) defined by

\[ x = x\left( u,v \right), \quad y = y\left( u,v \right) \]

How to integrate with \( \left( u,v \right) \)?

\begin{definition}
	The \textit{jacobian determinant} is defined by

	\[ J\left( u,v \right) = \left| \begin{bmatrix}
			\frac{\partial x}{\partial u} & \frac{\partial x}{\partial v} \\
			\frac{\partial y}{\partial u} & \frac{\partial y}{\partial v}
		\end{bmatrix} \right| = \frac{\partial x}{\partial u}\cdot \frac{\partial y}{\partial v} - \frac{\partial x}{\partial v} \cdot  \frac{\partial y}{\partial u} \]
\end{definition}

\begin{eg}
	Consider the polar coordinates

	\[ x = r\cos\theta, \quad y = r\sin\theta \]

	We want to compute \( J\left( r,\theta \right) \), we have

	\[ J\left( r,\theta \right) = \left| \begin{bmatrix}
			\frac{\partial x}{\partial r} & \frac{\partial x}{\partial \theta} \\
			\frac{\partial y}{\partial r} & \frac{\partial y}{\partial \theta}
		\end{bmatrix} \right| = \left| \begin{bmatrix}
			\cos\theta & -r\sin\theta \\
			\sin\theta & r\cos\theta
		\end{bmatrix} \right| \]

	We obtain

	\begin{align*}
		J\left( r,\theta \right) & = \cos\theta \cdot r\cos\theta - \sin\theta \cdot \left( -r\sin\theta \right) \\
		                         & = r\left( \left( \cos\theta \right)^2+\left( \sin\theta \right)^2 \right)     \\
		                         & = r
	\end{align*}

	This correspons to \( r \) in \( dA = rd\theta dr \).
\end{eg}

The determinant should be intepreted as an area (up to certain signs).

\begin{eg}
	Given \( \vec{v}=\left( a,b \right) \) and \( \vec{u}=\left( 0,d \right) \), consider \( \left( 0,0 \right) \), \( \vec{v}=\left( a,b \right) \), \( \vec{w}=\left( 0,d \right) \), \( \vec{v}+\vec{w} = \left( a,b+d \right) \). These four points define a paralellogram.


	\begin{figure}[H]
		\centering
		\incfig{paralellogram}
	\end{figure}
\end{eg}

we claim that

\[ a = \left| \text{ det} \begin{pmatrix}
		a & b \\
		0 & d
	\end{pmatrix} \right| = \left| ad \right| \]

we consider \( a, b, d > 0 \), then

\[ a = a\left( b+d \right) - \frac{1}{2} ab = \frac{1}{2} ab = ad \]

this is the same as the determinant. more generally, with

\[ \left( 0,0 \right), \vec{v}=\left( a,b \right), \quad \vec{w} = \left( c,d \right), \quad \vec{v}+\vec{w}=\left( a+c, b+d \right) \]

\[ \left| \text{ det} \begin{pmatrix}
		a & b \\
		c & d
	\end{pmatrix} \right| = \left| ab-bc \right| \]

the idea of change of variables can be described by the following figure.


\begin{figure}[h]
	\centering
	\incfig{changevariables}
\end{figure}
\[  \]
\begin{theorem}
	Change of variables.
	\medskip

	Let \( R \) be a region in cartesian coordinates


	\begin{figure}[H]
		\centering
		\incfig{cartesiancoors}
	\end{figure}

	Let \( S \) be the corresponding region in \( \left( u,v \right) \)-coordinates, then

	\[ \iint_{R} fdA = \iint_{S}f\left( x\left( u,v \right),y\left( u,v \right) \right)\left| J\left( u,v \right) \right|dudv \]
\end{theorem}


\end{document}
