\documentclass{article}
        \input{preamble.tex}

\begin{document}
\section{Lecture 9}

\subsection{Normal Vectors - Continued}

Yesterday we saw that

\[ \vec{N}\left( t \right) = \frac{\frac{d \vec{T}}{dt}}{\left| \frac{d \vec{T}}{dt} \right|} \]

\begin{figure}[H]
	\centering
	\def\svgwidth{0.6\textwidth}
	\import{./figures/}{fig19.pdf_tex}
\end{figure}

asdfasdfasdfas
\begin{eg}
	Consider the circle

	\[ \vec{r}\left( t \right) = \left( \cos t, \sin t \right), 0 \leq t \leq 2\pi \]

	The velocity is

	\[ \vec{v}\left( t \right) = \vec{r}'  = \left( -\sin t , \cos t \right)\]

	We have \( \left| \vec{v}\left( t \right) \right| = 1 \), since

	\[ \vec{v}\left( t \right)\cdot \vec{v}\left( t \right) = \left( \sin t^2 = \cos t^2 \right) =1\]

	We find that \( \vec{T}\left( t \right) = \vec{v}\left( t \right) \). To find \( \vec{N} \), we need first

	\[ \frac{d \vec{T}}{dt} = \frac{d \vec{v}}{dt} = \left( -\cos t, - \sin t \right) \]

	We check that \( \left| \frac{d \vec{T}}{dt} \right| = 1 \), then

	\[ \vec{N}\left( t \right) = \left( -\cos t, - \sin t \right) = -\vec{r}\left( t \right) \]

	We compute more explicitly:

	\[ \vec{N}\left( t \right)\cdot \vec{T}\left( t \right) = \left( -\cos t, -\sin t \right) \cdot  \left( -\sin t, \cos t \right) = \cos t \cdot  \sin t - \sin t \cdot  \cos t = 0 \]
	\begin{figure}[H]
		\centering
		\def\svgwidth{1\textwidth}
		\import{./figures/}{fig21.pdf_tex}
	\end{figure}

	We revisit the implicit case \( f\left( x,y \right)= 0 \).

	\begin{prop}

	\end{prop}


	\begin{proof}

	\end{proof}



\end{eg}

\end{document}
\documentclass{article}
\input{preamble.tex}

\begin{document}
\section{Lecture 9}

\subsection{Normal Vectors - Continued}

Yesterday we saw that

\[ \vec{N}\left( t \right) = \frac{\frac{d \vec{T}}{dt}}{\left| \frac{d \vec{T}}{dt} \right|} \]

\begin{figure}[H]
	\centering
	\def\svgwidth{0.6\textwidth}
	\import{./figures/}{fig19.pdf_tex}
\end{figure}

asdfasdfasdfas
\begin{eg}
	Consider the circle

	\[ \vec{r}\left( t \right) = \left( \cos t, \sin t \right), 0 \leq t \leq 2\pi \]

	The velocity is

	\[ \vec{v}\left( t \right) = \vec{r}'  = \left( -\sin t , \cos t \right)\]

	We have \( \left| \vec{v}\left( t \right) \right| = 1 \), since

	\[ \vec{v}\left( t \right)\cdot \vec{v}\left( t \right) = \left( \sin t^2 = \cos t^2 \right) =1\]

	We find that \( \vec{T}\left( t \right) = \vec{v}\left( t \right) \). To find \( \vec{N} \), we need first

	\[ \frac{d \vec{T}}{dt} = \frac{d \vec{v}}{dt} = \left( -\cos t, - \sin t \right) \]

	We check that \( \left| \frac{d \vec{T}}{dt} \right| = 1 \), then

	\[ \vec{N}\left( t \right) = \left( -\cos t, - \sin t \right) = -\vec{r}\left( t \right) \]

	We compute more explicitly:

	\[ \vec{N}\left( t \right)\cdot \vec{T}\left( t \right) = \left( -\cos t, -\sin t \right) \cdot  \left( -\sin t, \cos t \right) = \cos t \cdot  \sin t - \sin t \cdot  \cos t = 0 \]
	\begin{figure}[H]
		\centering
		\def\svgwidth{1\textwidth}
		\import{./figures/}{fig21.pdf_tex}
	\end{figure}

	We revisit the implicit case \( f\left( x,y \right)= 0 \).

	\begin{prop}

	\end{prop}


	\begin{proof}

	\end{proof}



\end{eg}

\end{document}
\documentclass{article}
\input{preamble.tex}

\begin{document}
\section{Lecture 9}

\subsection{Normal Vectors - Continued}

Yesterday we saw that

\[ \vec{N}\left( t \right) = \frac{\frac{d \vec{T}}{dt}}{\left| \frac{d \vec{T}}{dt} \right|} \]

\begin{figure}[H]
	\centering
	\def\svgwidth{0.6\textwidth}
	\import{./figures/}{fig19.pdf_tex}
\end{figure}

asdfasdfasdfas
\begin{eg}
	Consider the circle

	\[ \vec{r}\left( t \right) = \left( \cos t, \sin t \right), 0 \leq t \leq 2\pi \]

	The velocity is

	\[ \vec{v}\left( t \right) = \vec{r}'  = \left( -\sin t , \cos t \right)\]

	We have \( \left| \vec{v}\left( t \right) \right| = 1 \), since

	\[ \vec{v}\left( t \right)\cdot \vec{v}\left( t \right) = \left( \sin t^2 = \cos t^2 \right) =1\]

	We find that \( \vec{T}\left( t \right) = \vec{v}\left( t \right) \). To find \( \vec{N} \), we need first

	\[ \frac{d \vec{T}}{dt} = \frac{d \vec{v}}{dt} = \left( -\cos t, - \sin t \right) \]

	We check that \( \left| \frac{d \vec{T}}{dt} \right| = 1 \), then

	\[ \vec{N}\left( t \right) = \left( -\cos t, - \sin t \right) = -\vec{r}\left( t \right) \]

	We compute more explicitly:

	\[ \vec{N}\left( t \right)\cdot \vec{T}\left( t \right) = \left( -\cos t, -\sin t \right) \cdot  \left( -\sin t, \cos t \right) = \cos t \cdot  \sin t - \sin t \cdot  \cos t = 0 \]
	\begin{figure}[H]
		\centering
		\def\svgwidth{1\textwidth}
		\import{./figures/}{fig21.pdf_tex}
	\end{figure}

	We revisit the implicit case \( f\left( x,y \right)= 0 \).

	\begin{prop}

	\end{prop}


	\begin{proof}

	\end{proof}



\end{eg}

\end{document}
\documentclass{article}
\input{preamble.tex}

\begin{document}
\section{Lecture 9}

\subsection{Normal Vectors - Continued}

Yesterday we saw that

\[ \vec{N}\left( t \right) = \frac{\frac{d \vec{T}}{dt}}{\left| \frac{d \vec{T}}{dt} \right|} \]

\begin{figure}[H]
	\centering
	\def\svgwidth{0.6\textwidth}
	\import{./figures/}{fig19.pdf_tex}
\end{figure}

asdfasdfasdfas
\begin{eg}
	Consider the circle

	\[ \vec{r}\left( t \right) = \left( \cos t, \sin t \right), 0 \leq t \leq 2\pi \]

	The velocity is

	\[ \vec{v}\left( t \right) = \vec{r}'  = \left( -\sin t , \cos t \right)\]

	We have \( \left| \vec{v}\left( t \right) \right| = 1 \), since

	\[ \vec{v}\left( t \right)\cdot \vec{v}\left( t \right) = \left( \sin t^2 = \cos t^2 \right) =1\]

	We find that \( \vec{T}\left( t \right) = \vec{v}\left( t \right) \). To find \( \vec{N} \), we need first

	\[ \frac{d \vec{T}}{dt} = \frac{d \vec{v}}{dt} = \left( -\cos t, - \sin t \right) \]

	We check that \( \left| \frac{d \vec{T}}{dt} \right| = 1 \), then

	\[ \vec{N}\left( t \right) = \left( -\cos t, - \sin t \right) = -\vec{r}\left( t \right) \]

	We compute more explicitly:

	\[ \vec{N}\left( t \right)\cdot \vec{T}\left( t \right) = \left( -\cos t, -\sin t \right) \cdot  \left( -\sin t, \cos t \right) = \cos t \cdot  \sin t - \sin t \cdot  \cos t = 0 \]
	\begin{figure}[H]
		\centering
		\def\svgwidth{1\textwidth}
		\import{./figures/}{fig21.pdf_tex}
	\end{figure}

	We revisit the implicit case \( f\left( x,y \right)= 0 \).

	\begin{prop}

	\end{prop}


	\begin{proof}

	\end{proof}



\end{eg}

\end{document}

